An attempt at a more principled layout in specs/. One proof suddenly demanded 1 fuel; a proof that went through with default settings now wants 300 rlimit; two proofs in HMAC seem to have irrevocably broken and I can't revive them

specs/Spec.MD5.fst
@@ -3,7 +3,7 @@ module Spec.MD5
 (* Source: https://tools.ietf.org/html/rfc1321 *)
 
 module U32 = FStar.UInt32
-open Spec.Hash.Helpers
+open Spec.Hash.Definitions
 
 (* Section 3.3 *)
 
@@ -302,8 +302,8 @@ let update = update_aux
 
 (* Sections 3.1 and 3.2 *)
 
-let pad = Spec.Hash.Common.pad MD5
+let pad = Spec.Hash.PadFinish.pad MD5
 
 (* Section 3.5 *)
 
-let finish = Spec.Hash.Common.finish _
+let finish = Spec.Hash.PadFinish.finish _
