code/hash/Hacl.Hash.PadFinish.fst
@@ -7,10 +7,10 @@ module U128 = FStar.UInt128
 
 module Cast = FStar.Int.Cast.Full
 module Constants = Spec.SHA2.Constants
-module Helpers = Spec.Hash.Helpers
+module Helpers = Spec.Hash.Definitions
 module Endianness = FStar.Kremlin.Endianness
 module Math = FStar.Math.Lemmas
-module Helpers = Spec.Hash.Helpers
+module Helpers = Spec.Hash.Definitions
 
 module M = LowStar.Modifies
 module S = FStar.Seq
@@ -22,7 +22,8 @@ module ST = FStar.HyperStack.ST
 open LowStar.BufferOps
 open Hacl.Hash.Definitions
 open Hacl.Hash.Lemmas
-open Spec.Hash.Helpers
+open Spec.Hash.Definitions
+open Spec.Hash.Lemmas0
 
 (** Padding *)
 
