providers/evercrypt/fst/EverCrypt.Hash.Incremental.fst
@@ -14,7 +14,7 @@ module G = FStar.Ghost
 module Hash = EverCrypt.Hash
 
 open FStar.HyperStack.ST
-open Spec.Hash.Helpers
+open Spec.Hash.Definitions
 open FStar.Integers
 
 #reset-options "--max_fuel 0 --max_ifuel 0 --z3refresh \
@@ -47,7 +47,7 @@ let create_in a r =
   Hash.init #(G.hide a) hash_state;
 
   let h3 = ST.get () in
-  Spec.Hash.update_multi_zero a (Hash.repr hash_state h3);
+  Spec.Hash.Lemmas.update_multi_zero a (Hash.repr hash_state h3);
   split_at_last_empty a;
   assert (Hash.invariant hash_state h3);
   assert (v 0ul <= B.length buf);
@@ -398,8 +398,8 @@ let mk_finish a s prev dst =
   EverCrypt.Hash.finish #(G.hide a) tmp_hash_state dst;
 
   let h5 = ST.get () in
-  Spec.Hash.Incremental.hash_is_hash_incremental a (G.reveal prev);
-  assert (S.equal (B.as_seq h5 dst) (Spec.Hash.Nist.hash a (G.reveal prev)));
+  Spec.Hash.Lemmas.hash_is_hash_incremental a (G.reveal prev);
+  assert (S.equal (B.as_seq h5 dst) (Spec.Hash.hash a (G.reveal prev)));
 
   B.modifies_inert_intro (B.loc_buffer dst) h4 h5;
   Hash.frame_invariant (B.loc_buffer dst) hash_state h4 h5;
