specs/derived/Spec.Hash.Incremental.fst
@@ -1,0 +1,32 @@
+module Spec.Hash.Incremental
+
+module S = FStar.Seq
+
+open Spec.Hash
+open Spec.Hash.Definitions
+open Spec.Hash.PadFinish
+
+#set-options "--max_fuel 0 --max_ifuel 0 --z3rlimit 300"
+
+(* An incremental specification better suited to a stateful API, allowing the
+   client to perform the padding at the last minute upon hitting the last chunk of
+   data. *)
+let update_last (a:hash_alg)
+  (hash:hash_w a)
+  (prevlen:nat{prevlen % size_block a = 0})
+  (input:bytes{S.length input + prevlen < max_input8 a}):
+  Tot (hash_w a)
+=
+  let total_len = prevlen + S.length input in
+  let padding = pad a total_len in
+  update_multi a hash S.(input @| padding)
+
+let hash_incremental (a:hash_alg) (input:bytes{S.length input < (max_input8 a)}):
+  Tot (hash:bytes{S.length hash = (size_hash a)})
+=
+  let open FStar.Mul in
+  let n = S.length input / (size_block a) in
+  let bs, l = S.split input (n * (size_block a)) in
+  let hash = update_multi a (init a) bs in
+  let hash = update_last a hash (n * (size_block a)) l in
+  finish a hash
