specs/tests/Spec.Hash.Test.fst
@@ -208,8 +208,8 @@ let test5_expected224 = []
 //   0x4euy; 0xaduy; 0xb2uy; 0x17uy; 0xaduy; 0x8cuy; 0xc0uy; 0x9buy
 // ]
 
-open Spec.Hash.Nist
-open Spec.Hash.Helpers
+open Spec.Hash
+open Spec.Hash.Definitions
 
 //
 // Main
